more fiddling around with abstractbdd - this is all so intractible

thy/AbstractBDD.thy
@@ -13,55 +13,92 @@ record abdd =
 	nodes :: "abdd_node set"
 	start :: nodelabel
 
-definition abdd_reference_integrity :: "abdd \<Rightarrow> bool" where
-"abdd_reference_integrity b \<equiv> (\<forall>n \<in> nodes b.
+definition abdd_reference_integrity_set :: "abdd \<Rightarrow> bool" where
+"abdd_reference_integrity_set b \<equiv> (\<forall>n \<in> nodes b.
 	(\<forall>m \<in> nodes b. (label m = label n) \<longrightarrow> (m = n)) \<and> (
 	case (label n) of 
 		LabeledNode _ \<Rightarrow> ((\<exists>l \<in> nodes b. label l = left n) \<and> (\<exists>l \<in> nodes b. label l = right n)) |
 		_ \<Rightarrow> True))"
-
+definition "abdd_collect_refs bdd = {start bdd} \<union> right ` nodes bdd \<union> left ` nodes bdd"
+definition abdd_reference_integrity :: "abdd \<Rightarrow> bool" where
+	"abdd_reference_integrity bdd \<equiv> (\<forall>lb \<in> abdd_collect_refs bdd. \<exists>node \<in> nodes bdd. label node = lb)"
+definition abdd_nodes_unique :: "abdd \<Rightarrow> bool" where
+	"abdd_nodes_unique bdd \<equiv> (\<forall>n \<in> nodes bdd. (\<forall>m \<in> nodes bdd. (label m = label n) \<longrightarrow> (m = n)))"
+		
 definition "abddn_is_child c n \<equiv> (label c = left n \<or> label c = right n)" 
 inductive abdd_reachable :: "abdd \<Rightarrow> abdd_node \<Rightarrow> abdd_node \<Rightarrow> bool" where
 ar_base: "ln2 \<in> nodes bdd \<Longrightarrow> abddn_is_child ln2 ln  \<Longrightarrow> abdd_reachable bdd ln ln2" |
 ar_step: "ln2 \<in> nodes bdd \<Longrightarrow> abdd_reachable bdd ln ln2 \<Longrightarrow> abddn_is_child ln3 ln2  \<Longrightarrow> abdd_reachable bdd ln ln3"
+code_pred abdd_reachable .
 definition "abdd_reachable_set bdd node = {n |n. abdd_reachable bdd node n}"
+definition "abdd_cycle_free bdd = (\<forall>node \<in> nodes bdd. \<not> abdd_reachable bdd node node)"
 
 definition abdd_is_dag :: "abdd \<Rightarrow> bool" where
 "abdd_is_dag bdd = (\<forall>n \<in> nodes bdd. \<not>abdd_reachable bdd n n)"
 
-definition "getnode bdd lbl \<equiv> THE node. node \<in> nodes bdd \<and> label node = lbl"
-lemma "abdd_reference_integrity bdd \<Longrightarrow> node \<in> nodes bdd \<Longrightarrow>
-	(case label node of LabeledNode _ \<Rightarrow> True | _ \<Rightarrow> False) \<Longrightarrow> getnode bdd (right node) \<in> nodes bdd"
-unfolding abdd_reference_integrity_def getnode_def
-apply(cases "label node") defer apply auto[2]
-apply clarsimp
-apply(rule the1I2) defer apply simp
-find_theorems "\<exists>!x . _"
-apply(rule ex1I)
-thm ex1I
-oops
-
-function abstract_abdd_hlp :: "abdd \<Rightarrow> abdd_node \<Rightarrow> boolfunc" where
-"abstract_abdd_hlp bdd node l = (if (abdd_is_dag bdd \<and> abdd_reference_integrity bdd)
-	then (if l ! var node 
-		then abstract_abdd_hlp bdd (getnode bdd (right node)) l 
-		else abstract_abdd_hlp bdd (getnode bdd (left node)) l)
-	else undefined)"
-by pat_completeness auto
-
 lemma "abdd_is_dag bdd \<Longrightarrow>
        (*abdd_reference_integrity bdd \<Longrightarrow>*) 
        abdd_reachable_set bdd (getnode bdd (right node)) \<subseteq> (abdd_reachable_set bdd node)"
-apply(rule, unfold abdd_reachable_set_def, simp) oops
-
-termination abstract_abdd_hlp
-apply(relation "measure (card \<circ> (\<lambda>(bdd,node,_). abdd_reachable_set bdd node))", rule wf_measure, unfold in_measure comp_def)
-(*apply(unfold getnode_def abdd_reference_integrity_def abdd_reachable_set_def)*)
-apply clarsimp
-apply(rule psubset_card_mono) defer
-apply(rule, rule, unfold abdd_reachable_set_def, simp)[1]
+apply(rule, unfold abdd_reachable_set_def, simp)
 oops
 
+definition "abdd_terminal state = (case state of LabeledNode _ \<Rightarrow> False | _ \<Rightarrow> True)" 
+
+inductive abdd_smallstep  where
+start: "abdd_smallstep bdd assignment (start bdd)" |
+step[elim]: "abdd_smallstep bdd assignment state \<Longrightarrow> \<not> abdd_terminal state \<Longrightarrow> node \<in> nodes bdd \<Longrightarrow> label node = state \<Longrightarrow> abdd_smallstep bdd assignment ((if assignment ! var node then right else left) node)"
+print_theorems
+code_pred abdd_smallstep .
+inductive abdd_smallstep2  where
+start: "abdd_smallstep2 bdd assignment (start bdd)" |
+stepright: "abdd_smallstep2 bdd assignment state \<Longrightarrow> \<not> abdd_terminal state \<Longrightarrow> node \<in> nodes bdd \<Longrightarrow> label node = state \<Longrightarrow> assignment ! var node \<Longrightarrow> abdd_smallstep2 bdd assignment (right node)" |
+stepleft: "abdd_smallstep2 bdd assignment state \<Longrightarrow> \<not> abdd_terminal state \<Longrightarrow> node \<in> nodes bdd \<Longrightarrow> label node = state \<Longrightarrow> \<not>assignment ! var node \<Longrightarrow> abdd_smallstep2 bdd assignment (left node)"
+lemma abdd_smallstep_2_eq: "abdd_smallstep bdd ass state = abdd_smallstep2 bdd ass state"
+	apply(rule)
+	 apply(induction rule: abdd_smallstep.induct)
+	  apply(simp add: abdd_smallstep2.start)
+	 apply(force dest: abdd_smallstep2.stepright abdd_smallstep2.stepleft)
+	apply(induction rule: abdd_smallstep2.induct)
+	  apply(simp add: abdd_smallstep.start)
+	 apply(force dest: abdd_smallstep.step)
+	apply(force dest: abdd_smallstep.step)
+done
+
+definition "abdd_xor \<equiv> \<lparr> nodes = {
+	\<lparr> var = 0, label = LabeledNode 5, right = LabeledNode 4 , left = LabeledNode 3 \<rparr>,
+	\<lparr> var = 1, label = LabeledNode 4, right = DFalse , left = DTrue \<rparr>,
+	\<lparr> var = 1, label = LabeledNode 3, right = DTrue , left = DFalse \<rparr>,
+	\<lparr> var = 0, label = DTrue , right = DTrue , left = DTrue \<rparr>,
+	\<lparr> var = 0, label = DFalse , right = DFalse , left = DFalse \<rparr>
+}, start = LabeledNode 5\<rparr>"
+
+lemma "abdd_reference_integrity abdd_xor" by eval
+lemma "abdd_cycle_free abdd_xor" unfolding abdd_cycle_free_def apply(subst abdd_xor_def, simp) apply(rule) oops 
+lemma "abdd_smallstep abdd_xor [False, True] DTrue" 
+proof -
+	have 1: "abdd_smallstep abdd_xor [False, True] (start abdd_xor)" by(simp add: abdd_smallstep.start)
+	have 2: "\<lparr> var = 0, label = LabeledNode 5, right = LabeledNode 4 , left = LabeledNode 3 \<rparr> \<in> nodes abdd_xor" by(simp add: abdd_xor_def)
+	have 3: "abdd_smallstep abdd_xor [False, True] (LabeledNode 3)" using abdd_smallstep.step[OF 1 _ 2] by(simp add: abdd_xor_def abdd_terminal_def)
+	have 4: "\<lparr> var = 1, label = LabeledNode 3, right = DTrue , left = DFalse \<rparr> \<in> nodes abdd_xor" by(simp add: abdd_xor_def)
+	show 5: "abdd_smallstep abdd_xor [False, True] DTrue" using abdd_smallstep.step[OF 3 _ 4] by(simp add: abdd_xor_def abdd_terminal_def)
+qed (* So how do I do this automatically? *)
+values "{t|t. abdd_smallstep2 abdd_xor [False, True] t}" (* I guess I don't? *)
+
+definition "abstract_abdd1 bdd ass = (
+	if abdd_smallstep bdd ass DTrue
+		then Some True else (
+	if abdd_smallstep bdd ass DFalse
+		then Some False
+	else None))"
+
+lemma abdd_steppable_ind: " (\<exists>node \<in> nodes bdd. label node = state)
+	\<Longrightarrow> abdd_smallstep bdd ass state \<Longrightarrow> (\<exists>nextnode \<in> nodes bdd. abdd_smallstep bdd ass (label nextnode))" by blast
+
+
+lemma "abdd_reference_integrity bdd \<Longrightarrow> abdd_cycle_free bdd \<Longrightarrow> abstract_abdd1 bdd ass \<noteq> None"
+apply(unfold abstract_abdd1_def)
+apply(unfold abdd_smallstep_2_eq)
+oops
 
 
 end
